Add a BBM success test case (with DSB, ISB, TLBI) (#46)
- Update sail-tiny-arm commit hash
- Refactor tests

ArchSemArm/tests/VMPromisingTest.v
@@ -513,7 +513,7 @@ Module MPDMBS.
 End MPDMBS.
 
 (* Sequential page table modification in single thread *)
-Module BBM.
+Module BBMFailure.
   (* Single thread that:
      1. Loads from VA 0x8000001000 (gets 0x2a from PA 0x1000)
      2. Modifies L3[1] to remap VA 0x8000001000 -> PA 0x2000
@@ -587,4 +587,99 @@ Module BBM.
     vm_compute (elements _).
     apply NoDup_Permutation; try solve_NoDup; set_solver.
   Qed.
-End BBM.
+End BBMFailure.
+
+(* Break-before-make success case *)
+Module BBMSuccess.
+  (* Thread 0:
+      - updates the last-level PTE for VA 0x8000001000
+      - executes a break-before-make sequence that only
+        invalidates the last-level mapping for that VA:
+        DSB ISHST; TLBI VAE1IS, X0; DSB ISH.
+    Thread 1:
+      - performs a data access via VA 0x8000001000. *)
+
+  Definition init_reg_t1 : registerMap :=
+    ∅
+    |> reg_insert _PC 0x8000000500
+    |> reg_insert R0 0x8000001000    (* VA to load from *)
+    |> reg_insert R1 0x0
+    |> reg_insert R2 0x8000010008    (* VA of L3[1] descriptor *)
+    |> reg_insert R3 0x0
+    |> reg_insert SCTLR_EL1 0x1
+    |> reg_insert TCR_EL1 0x0
+    |> reg_insert TTBR0_EL1 0x80000
+    |> reg_insert ID_AA64MMFR1_EL1 0x0
+    |> reg_insert PSTATE (init_pstate 1%bv 1%bv).
+
+  Definition init_reg_t2 : registerMap :=
+    ∅
+    |> reg_insert _PC 0x8000000600
+    |> reg_insert R0 0x8000001000    (* VA to load from *)
+    |> reg_insert R1 0x0
+    |> reg_insert SCTLR_EL1 0x1
+    |> reg_insert TCR_EL1 0x0
+    |> reg_insert TTBR0_EL1 0x80000
+    |> reg_insert ESR_EL1 0x0
+    |> reg_insert ID_AA64MMFR1_EL1 0x0
+    |> reg_insert PSTATE (init_pstate 1%bv 1%bv).
+
+  (* T1 Instructions *)
+  Definition init_mem :=
+    ∅
+    (* Instructions T1 *)
+    |> mem_insert 0x500 4 0xf8226823 (* STR X3, [X1, X2] - invalidate the PTE *)
+    |> mem_insert 0x504 4 0xd5033a9f (* DSB ISHST *)
+    |> mem_insert 0x508 4 0xd5088320 (* TLBI VAE1IS, X0 *)
+    |> mem_insert 0x50C 4 0xd5033b9f (* DSB ISH *)
+    |> mem_insert 0x510 4 0xd5033fdf (* ISB *)
+    (* Instructions T2 *)
+    |> mem_insert 0x600 4 0xf8606820 (* LDR X0, [X1, X0] - read 0x8000001000 *)
+    (* Data *)
+    |> mem_insert 0x1000 8 0x2a
+    (* Page Tables *)
+    |> mem_insert 0x80008 8 0x81803
+    |> mem_insert 0x81000 8 0x82003
+    |> mem_insert 0x82000 8 0x83003
+    |> mem_insert 0x83000 8 0x40000000000783
+    |> mem_insert 0x83008 8 0x60000000001783
+    |> mem_insert 0x83080 8 0x60000000083703.
+
+  Definition n_threads := 2%nat.
+
+  Definition terminate_at_t1 rm : bool :=
+    reg_lookup _PC rm =? Some (0x800000050C : bv 64).
+
+  Definition terminate_at_t2 rm : bool :=
+    (* a valid translation *)
+    (reg_lookup _PC rm =? Some (0x8000000604 : bv 64))
+    (* or a fault *)
+    || ((reg_lookup FAR_EL1 rm =? Some (0x8000001000 : bv 64))
+        && (reg_lookup ELR_EL1 rm =? Some (0x8000000600 : bv 64))
+        && (reg_lookup ESR_EL1 rm =? Some (0x96000007 : bv 64))).
+
+  Definition terminate_at := [# terminate_at_t1; terminate_at_t2].
+
+  Definition termCond : terminationCondition n_threads :=
+    (λ tid rm, (terminate_at !!! tid) rm).
+
+  Definition fuel := 8%nat.
+  Definition debug := true.
+  Definition mem_strict := false.
+
+  Definition initState :=
+    {|archState.memory := init_mem;
+      archState.regs := [# init_reg_t1; init_reg_t2];
+      archState.address_space := PAS_NonSecure |}.
+
+  Definition test_results :=
+    VMPromising_cert_c_pf arm_sem fuel debug mem_strict n_threads termCond initState.
+
+  (* BBM check success *)
+  Goal elements (regs_extract [(1%fin, R0)] <$> test_results) ≡ₚ
+      [Ok [0x2a%Z]].
+  Proof.
+    vm_compute (elements _).
+    apply NoDup_Permutation; try solve_NoDup; set_solver.
+  Qed.
+End BBMSuccess.
